Version with compiling reduction

krivineAM.v
@@ -21,7 +21,7 @@ with code: Type :=
 
 Inductive environment : Type := 
 | nul: environment
-| cons: (prod code environment) -> environment -> environment.
+| cons: code -> environment -> environment -> environment.
 
 Check environment_ind.
 
@@ -36,16 +36,16 @@ Check Set -> Type.
 Check environment.
 Check environment_ind.
 
-Check cons (cnil,nul) nul.
+Check cons  cnil nul nul.
 
 (*Semantics*)
 
-Fixpoint exec_inst (s: state): state:=
+Definition exec_inst (s: state): state:=
   match s with
-    | (cCons (Access 0) c, cons (c0,e0) e, stack) => (c0, e0, stack)
-    | (cCons (Access n) c, cons (c0,e0) e, stack) => (cCons (Access (n-1)) c, e, stack)
-    | (cCons (Push c) c0, e, stack) => (c0, e, cons (c,e) stack)
-    | (cCons Grab c, e, cons (c0,e0) stack) => (c, cons (c0,e0) e, stack)
+    | (cCons (Access 0) c, cons c0 e0 e, stack) => (c0, e0, stack)
+    | (cCons (Access n) c, cons c0 e0 e, stack) => (cCons (Access (n-1)) c, e, stack)
+    | (cCons (Push c) c0, e, stack) => (c0, e, cons c e stack)
+    | (cCons Grab c, e, cons  c0 e0 stack) => (c, cons c0 e0 e, stack)
     | s => s
   end.
 
@@ -72,7 +72,7 @@ Check multiple_substitution.
 Fixpoint tau_env (e: environment): list term :=
   match e with
     | nul => nil
-    | cons (c0, e0) e1 =>
+    | cons c0 e0 e1 =>
       (multiple_substitution 0 (tau_code c0) (tau_env e0)) :: tau_env e1
   end.
 
@@ -80,8 +80,8 @@ Check state.
 
 Fixpoint transform_stk (stk: environment): list term :=
   match stk with
-      | cons (c0, e0) nul => multiple_substitution 0 (tau_code c0) (tau_env e0) :: nil
-      | cons (c0, e0) e1 => (multiple_substitution 0 (tau_code c0) (tau_env e0)) :: (transform_stk e1)
+      | cons c0 e0 nul => multiple_substitution 0 (tau_code c0) (tau_env e0) :: nil
+      | cons c0 e0 e1 => (multiple_substitution 0 (tau_code c0) (tau_env e0)) :: (transform_stk e1)
       | nul => nil
   end.
 
@@ -176,7 +176,7 @@ Qed.
 Fixpoint lenEnv (e: environment): nat :=
   match e with
     | nul => 0
-    | cons (c0, e0) e1 => 1 + (lenEnv e1)
+    | cons c0 e0 e1 => 1 + (lenEnv e1)
   end.
 
 
@@ -186,76 +186,76 @@ Proof.
   induction e.
   done.
   Search "ective_pair".
-  rewrite (surjective_pairing p).
   simpl.
   omega.
 Qed.
 
 
-Fixpoint correct_stk (stk: environment): Prop:=
-  match stk with
-    | nul => True
-    | cons (c0, e0) e => (correct_stk e0) /\ (correct_stk e) /\ (C (lenEnv e0) (tau_code c0)) 
-  end.
+Inductive correct_stk : environment -> Prop :=
+| Correct_stk_nil : correct_stk nul
+| Correct_stk : forall (c0: code) (e0 e: environment),
+                  C (lenEnv e0) (tau_code c0) -> correct_stk e0 -> correct_stk e ->
+                  correct_stk (cons c0 e0 e).
 
-Fixpoint correct_state (s: state): Prop:=
+Definition correct_state (s: state): Prop:=
   match s with
    | (c, e, stk) => (correct_stk e) /\ (correct_stk stk) /\ (C (lenEnv e) (tau_code c))
   end.
 
-Theorem transition_inv_1: forall (c c0: code) (e e0 stack: environment), correct_state ((cCons (Access 0) c, cons (c0,e0) e, stack)) -> correct_state  (c0, e0, stack).
+Theorem transition_inv_1: forall (c c0: code) (e e0 stack: environment), correct_state ((cCons (Access 0) c, cons c0 e0 e, stack)) -> correct_state  (c0, e0, stack).
 Proof.
   simpl.
   intros.
   split.
-  apply H.
+  destruct H.
+  inversion H; trivial.
   split.
   apply H.
-  apply H.
+  destruct H.
+  inversion H; trivial.
 Qed.
 
-Theorem transition_inv_2: forall (c c0: code) (e e0 stack: environment) (n: nat), (n > 0) -> correct_state (cCons (Access n) c, cons (c0,e0) e, stack) -> correct_state (cCons (Access (n-1)) c, e, stack).
+Theorem transition_inv_2: forall (c c0: code) (e e0 stack: environment) (n: nat), (n > 0) -> correct_state (cCons (Access n) c, cons c0 e0 e, stack) -> correct_state (cCons (Access (n-1)) c, e, stack).
 Proof.
   simpl.
   intros.
-  split.  
-  apply H0.
+  split.
+  destruct H0.
+  inversion H0; trivial.
   split.
   apply H0.
-  destruct H0.
-  destruct H1.
+  destruct H0 as [h0 [h1 h2]].
   omega.
 Qed.
 
-Theorem transition_inv_3: forall (c c0: code) (e stack: environment), correct_state (cCons (Push c) c0, e, stack) -> correct_state (c0, e, cons (c,e) stack).
+Theorem transition_inv_3: forall (c c0: code) (e stack: environment), correct_state (cCons (Push c) c0, e, stack) -> correct_state (c0, e, cons c e stack).
 Proof.
   simpl.  
   intros.
+  destruct H as [h1 [h2 [h3 h4]]].
+  split; trivial.
   split.
-  apply H.
-  split.
-  split.
-  apply H.
-  split.
-  apply H.
-  apply H.
-  apply H.  
+  apply Correct_stk.
+  done.
+  done.
+  done.
+  done.
 Qed.
 
-Theorem transition_inv_4: forall (c c0: code) (e e0 stack: environment), correct_state (cCons Grab c, e, cons (c0,e0) stack) -> correct_state (c, cons (c0,e0) e, stack).
+Theorem transition_inv_4: forall (c c0: code) (e e0 stack: environment), correct_state (cCons Grab c, e, cons c0 e0 stack) -> correct_state (c, cons c0 e0 e, stack).
 Proof.
   simpl.
   intros.
+  destruct H as [h1 [h2 h3]].
   split.
+  apply Correct_stk.
+  inversion h2.
+  done.
+  by (inversion h2).
+  trivial.
   split.
-  apply H.
-  split.
-  apply H.
-  apply H.
-  split.
-  apply H.
-  rewrite plus_comm in H.
-  apply H.
+  by (inversion h2).
+  by rewrite plus_comm in h3.
 Qed.
 
 Theorem correct_invariance: forall s: state, correct_state s -> correct_state (exec_inst s).
@@ -282,8 +282,7 @@ Proof.
   done.
   simpl.
   done.
-  intros p e1.
-  destruct p.
+  intros c0 e1 e2.
   unfold exec_inst.
   case n.
   apply transition_inv_1.
@@ -294,14 +293,13 @@ Proof.
   intros e e0.
   case e.
   done.
-  intros p e1.
-  destruct p.
+  intros c0 e1 e2.
   apply transition_inv_4.
   intros c0 e e0.
   apply transition_inv_3.
 Qed.
 
-Lemma correct_reduction_1: forall (c c0: code) (e s: environment), correct_state (cCons (Push c0) c,e,s) -> reduces (tau (cCons (Push c0) c,e,s)) (tau (c, e, cons (c0, e) s)).
+Lemma correct_reduction_1: forall (c c0: code) (e s: environment), correct_state (cCons (Push c0) c,e,s) -> reduces (tau (cCons (Push c0) c,e,s)) (tau (c, e, cons c0 e s)).
 Proof.
   intros.
   simpl.
@@ -309,13 +307,12 @@ Proof.
   simpl.
   apply sym.
   intros.
-  destruct p.
   simpl in H.
   simpl.
   apply sym.
 Qed.
 
-Lemma correct_reduction_2: forall (c c0: code) (e e0 s: environment),correct_state ((cCons (Access 0) c, cons (c0,e0) e, s)) -> reduces (tau (cCons (Access 0) c, cons (c0,e0) e, s)) (tau (c0, e0, s)).
+Lemma correct_reduction_2: forall (c c0: code) (e e0 s: environment),correct_state ((cCons (Access 0) c, cons c0 e0 e, s)) -> reduces (tau (cCons (Access 0) c, cons c0 e0 e, s)) (tau (c0, e0, s)).
 Proof.
   simpl.
   intros.
@@ -326,7 +323,7 @@ Proof.
 Qed.  
 
   
-Lemma correct_reduction_3: forall (c c0: code) (e e0 s: environment) (n: nat), (n > 0) -> correct_state (cCons (Access n) c, cons (c0,e0) e, s) -> reduces (tau (cCons (Access n) c, cons (c0,e0) e, s)) (tau (exec_inst (cCons (Access n) c, cons (c0,e0) e, s))).
+Lemma correct_reduction_3: forall (c c0: code) (e e0 s: environment) (n: nat), (n > 0) -> correct_state (cCons (Access n) c, cons c0 e0 e, s) -> reduces (tau (cCons (Access n) c, cons c0 e0 e, s)) (tau (exec_inst (cCons (Access n) c, cons c0 e0 e, s))).
 Proof.
   have:forall n:nat, beq_nat n n = true.
   intro.
@@ -369,7 +366,7 @@ Proof.
   intro.
   rewrite x1.
   apply sym.
-  intros; destruct p.
+  intros.
   unfold tau.
   rewrite NPeano.Nat.sub_succ.
   rewrite -minus_n_O.
@@ -383,7 +380,7 @@ Proof.
   intro.
   rewrite ?x.
   simpl in h3.
-  have: S n <= lenEnv (cons (c0,e0) e) - 1.
+  have: S n <= lenEnv (cons c0 e0 e) - 1.
   simpl.
   simpl in h3.
   rewrite -minus_n_O.
@@ -466,15 +463,60 @@ Proof.
   omega.
 Qed.
 
-Lemma lift_len_inv: forall (lu: list term) (i k: nat), Datatypes.length lu = Datatypes.length (lift_all i k lu).
+Lemma lift_len_inv: forall (lu: list term) (i k: nat), length lu = length (lift_all i k lu).
 Proof.
-  admit.
+  induction lu; simpl.
+  by simpl.
+  intros.
+  by rewrite -IHlu.
+Qed.
+
+Lemma remove_lift: forall (t: term) (i k: nat), C k t -> lifting i k t = t.
+Proof.
+  induction t; simpl.
+  intros.
+  have: leb k v = false.
+  by apply leb_iff_conv.
+  intros.
+  by rewrite x.
+  intros.
+  rewrite -lambda_equivalence.
+  by apply IHt.
+  intros.
+  rewrite app_equivalence.
+  split.
+  apply IHt1.
+  tauto.
+  apply IHt2.
+  tauto.
 Qed.
 
 
 Lemma list_lift_free: forall (lu : list term) (i k : nat), c_list_i i lu -> c_list_i (i + 1) (lift_all 1 k lu).
 Proof.
-  admit.
+  induction lu; simpl.
+  unfold c_list_i.
+  simpl.
+  intros.
+  omega.
+  unfold c_list_i.
+  intros i k h1 k0.
+  case k0.
+  simpl.
+  intro.
+  apply lift_free.
+  apply (h1 0).
+  simpl.
+  omega.
+  simpl.  
+  intros.
+  apply IHlu.
+  unfold c_list_i.
+  intros.  
+  apply (h1 (S k1)).
+  simpl.
+  omega.
+  omega.
 Qed.
 
 Lemma mult_sub_clos: forall (t: term) (u: list term) (i: nat), closed_list i u -> C (i+Datatypes.length u) t -> C i (multiple_substitution i t u).
@@ -533,125 +575,158 @@ Proof.
   done.
   tauto.  
 Qed.
-  
-(*Lemma mult_sub_clos: forall (t: term) (u: list term) (i: nat), c_list_i i u -> C (i+Datatypes.length u) t -> C i (multiple_substitution t u i (Datatypes.length u)).
-Proof.
-  induction t.
-  simpl.
-  intros.
-  have: beq_nat v v = true.
-  apply beq_nat_true_iff.
-  done.
-  intro.
-  rewrite x.
-  have:leb v (i + Datatypes.length u - 1) = true.
-  apply leb_iff.
-  omega.
-  intro.
-  rewrite x0.
-  rewrite Bool.andb_true_r.
-  have:leb i v = false \/ leb i v = true.
-  apply dic.
-  intro.
-  case x1.
-  intro.
-  rewrite H1.
-  simpl.
-  apply leb_iff_conv in H1.
-  trivial.
-  intro.
-  rewrite H1.
-  apply H.
-  apply leb_iff in H1.
-  omega.
-  simpl.
-  intros.
-  rewrite (lift_len_inv _ 1 0).
-  apply (IHt (lift_all 1 0 u) (i+1)).
-  apply list_lift_free.
-  done.
-  rewrite -(lift_len_inv _ 1 0).
-  have: i + Datatypes.length u + 1 = i + 1 + Datatypes.length u.
-  omega.
-  intro.
-  rewrite -x.
-  trivial.
-  simpl.
-  intros.
-  split.
-  apply IHt1.
-  done.
-  tauto.  
-  apply IHt2.
-  done.
-  tauto.  
-Qed.*)
-
 
 
 Lemma closed_env: forall e:environment, correct_stk e -> closed_list 0 (tau_env e).
 Proof.
   induction e.
   simpl.
+  intros.
   trivial.
-  destruct p.
-  simpl.
   intros.
+  simpl.
+  inversion H.
   split.
-  
-
-
-  
-Abort.
-
-Lemma closed_env: forall e:environment, correct_stk e -> c_list_i 0 (tau_env e).
-Proof.
-  induction e.
-  simpl.
-  unfold c_list_i.
-  intros.
-  simpl in H0.
-  omega.
-  destruct p; simpl.
-  intros.
-  unfold c_list_i.
-  intros.
-  simpl in H0.
-  case k.
-  simpl.
   apply mult_sub_clos.
-Abort.
-  
-Lemma correct_reduction_4: forall (c c0: code) (e e0 s: environment), correct_state (cCons Grab c, e, cons (c0,e0) s) -> reduces (tau (cCons Grab c, e, cons (c0,e0) s)) (tau (c, cons (c0,e0) e, s)).
+  by apply IHe1.
+  simpl.
+  by rewrite -length_inv.
+  by apply IHe2.
+Qed.
+
+Lemma remove_list_lift: forall lu: list term, closed_list 0 lu -> lift_all 1 0 lu = lu.
 Proof.
+  induction lu.
+  by simpl.
+  simpl.
   intros.
-  simpl in H.
-  destruct H as [h0 [h1 h2]].
-  destruct h1.
-  destruct H0.
-  case s.
-  unfold tau.
+  have: lifting 1 0 a = a.
+  apply remove_lift.
+  tauto.
+  intro.
+  rewrite x.
+  have: lift_all 1 0 lu = lu.
+  apply IHlu.
+  tauto.
+  intro.
+  by rewrite x0.
+Qed.
+
+Lemma fold_reduce: forall (s: environment) (t u: term), reducesInOneTo t u -> reduces (fold_left (fun t1 t2 : term => App t1 t2) (transform_stk s) t) (fold_left (fun t1 t2 : term => App t1 t2) (transform_stk s) u).
+Proof.
+  induction s.
+  intros t u.
+  simpl.
+  intro.
+  apply (ind t u u).
+  trivial.
+  apply sym.
+  intros.
   unfold transform_stk.
-  unfold fold_left.
+  fold transform_stk.
+  have: match s2 with
+        | nul => multiple_substitution 0 (tau_code c) (tau_env s1) :: nil
+        | cons _ _ _ =>
+            multiple_substitution 0 (tau_code c) (tau_env s1)
+            :: transform_stk s2
+        end = multiple_substitution 0 (tau_code c) (tau_env s1) :: match s2 with
+        | nul => nil
+        | cons _ _ _ => transform_stk s2
+        end.
+  by case s2.
+  intro.
+  rewrite x.
+  clear x.
+  have:forall t:term, (fold_left (fun t1 t2 : term => App t1 t2)
+        (multiple_substitution 0 (tau_code c) (tau_env s1)
+         :: match s2 with
+            | nul => nil
+            | cons _ _ _ => transform_stk s2
+            end) t)
+            =
+            (fold_left (fun t1 t2 : term => App t1 t2)
+                       match s2 with
+                         | nul => nil
+                         | cons _ _ _ => transform_stk s2
+                       end) (App t (multiple_substitution 0 (tau_code c) (tau_env s1))).
+  by case s2.
+  intros.
+  rewrite ?x.
+  clear x.
+  move:IHs2.
+  case s2.
+  simpl.
+  intros.
+  apply (ind _ (App u (multiple_substitution 0 (tau_code c) (tau_env s1))) _).
+  by apply appLeft.
+  apply sym.
+  intros.
+  apply IHs2.
+  by apply appLeft.
+Qed.
+
+Lemma correct_reduction_4: forall (c: code) (e s: environment), correct_state (cCons Grab c, e, s) -> reduces (tau (cCons Grab c, e, s)) (tau (exec_inst (cCons Grab c, e, s))).
+Proof.
+  intros c e s.
+  move: c e.
+  induction s.
+  simpl.
+  intros.
+  apply sym.
+  intros.
+  inversion H.
+  unfold exec_inst.
+  unfold tau.
   unfold tau_code.
   fold tau_code.
+  unfold transform_stk.
+  fold transform_stk.
+  have: match s2 with
+        | nul => multiple_substitution 0 (tau_code c) (tau_env s1) :: nil
+        | cons _ _ _ =>
+            multiple_substitution 0 (tau_code c) (tau_env s1)
+            :: transform_stk s2
+        end = multiple_substitution 0 (tau_code c) (tau_env s1) :: match s2 with
+        | nul => nil
+        | cons _ _ _ => transform_stk s2
+        end.
+  by case s2.
+  intro.
+  rewrite x.
+  unfold multiple_substitution.
+  fold multiple_substitution.
   simpl.
-  apply (ind _  (substitution 0 (multiple_substitution 1 (tau_code c) (lift_all 1 0 (tau_env e)))
-                                (multiple_substitution 0 (tau_code c0) (tau_env e0)))  _).
-  apply removeLamb.
   rewrite mult_sub_inv.
-  rewrite -?length_inv.
+  case s2.
   simpl.
-  unfold correct_stk in h0.
-  induction e.
-  simpl.
+  have:lift_all 1 0 (tau_env e) = tau_env e.
+  apply remove_list_lift.
+  by apply closed_env.
+  clear x.
+  intro.
+  rewrite x.
+  apply (ind _ (substitution 0 (multiple_substitution 1 (tau_code c0) (tau_env e))
+        (multiple_substitution 0 (tau_code c) (tau_env s1))) _).
+  apply removeLamb.
+  apply sym.
   intros.
-  admit.
-  admit.
-  admit.
-  admit.
+  apply fold_reduce.
+  simpl.  
+  have:lift_all 1 0 (tau_env e) = tau_env e.
+  apply remove_list_lift.
+  by apply closed_env.
+  clear x.
+  intro.
+  rewrite x.
+  apply removeLamb.
+  intro j.
+  apply closed_list_eq.
+  simpl in H.
+  destruct H as [h1 [h2 h3]].
+  by apply closed_env.  
 Qed.
-  
+
+
 Theorem correct_confluence: forall s: state, correct_state s -> reduces (tau s) (tau (exec_inst s)).
 Proof.
   intro s.
@@ -670,23 +745,17 @@ Proof.
   intro.
   apply sym.
   intros.
-  rewrite (surjective_pairing p).
   apply correct_reduction_2.
-  rewrite -(surjective_pairing p).
   done.
-
   case e.
   intros.
   unfold exec_inst.
   apply sym.
-  intros p e0 n0.
-  rewrite (surjective_pairing p).
+  intros c0 e0 e1 n0.
   intro.
   apply correct_reduction_3.
   omega.
   done.
-
-
   unfold exec_inst.
   intros.
   move:H.
@@ -694,10 +763,8 @@ Proof.
   intro.
   apply sym.
   intros.
-  destruct p.
   apply correct_reduction_4.
   done.
-
   unfold exec_inst.
   intros.
   apply correct_reduction_1.
